Map implementation

theories/Process.v
@@ -1,5 +1,40 @@
 From stdpp Require Import base.
+From Metaconfigurations.Syntax Require Import Value.
 
 Class Process (Π : Type) := {
   register_names : Π → Type;
+  eq_dec_register_names π (r r' : register_names π) : {r = r'} + {r ≠ r'};
 }.
+
+Module RegisterFile.
+  Section RF.
+
+    Context {Π : Type} `{Process Π}.
+
+    Variable (π : Π).
+
+    Definition t := register_names π → Value.t.
+
+    Definition rebind : register_names π → Value.t → t → t.
+    Proof.
+      intros r v m r'. destruct (eq_dec_register_names π r r').
+      - exact v.
+      - exact (m r').
+    Defined.
+
+    Definition lookup (r : register_names π) (m : t) : Value.t := m r.
+
+    Definition init : t := λ _, ⊤ᵥ.
+
+    Theorem lookup_rebind_same k v m : lookup k (rebind k v m) = v.
+    Proof.
+      unfold lookup, rebind. now destruct (eq_dec_register_names π k k).
+    Qed.
+
+    Theorem lookup_rebind_diff k k' v m : k ≠ k' → lookup k' (rebind k v m) = lookup k' m.
+    Proof.
+      intros. unfold lookup, rebind. now destruct (eq_dec_register_names π k k').
+    Qed.
+  End RF.
+
+End RegisterFile.
