theories/Statics/Value.v
@@ -1,12 +1,36 @@
 From stdpp Require Import base.
-Require Import Metaconfigurations.Syntax.Value.
+From stdpp Require Import base gmap.
+Require Import Metaconfigurations.Syntax.Ty.
+Require Import Coq.Classes.SetoidDec.
+Require Import Coq.ZArith.BinInt.
+Require Import Coq.Lists.List.
+Require Import Coq.Logic.Decidable.
+From Metaconfigurations.Syntax Require Import Value Ty.
 
-Inductive type : t → Ty.t → Prop :=
-  | type_int n : type (Int n) Ty.Int
-  | type_bool b : type (Bool b) Ty.Bool
-  | type_unit : type Unit Ty.Unit
-  | type_tuple vs τs : Forall2 type vs τs → type (Tuple vs) (Ty.Tuple τs).
+Reserved Notation "v :ᵥ τ" (at level 80, no associativity).
+
+Inductive type : Value.t → Ty.t → Prop :=
+  | type_int (n : Z) : n :ᵥ Ty.Int
+  | type_bool (b : bool) : b :ᵥ Ty.Bool
+  | type_unit : Value.Unit :ᵥ Ty.Unit
+  | type_tuple v₁ v₂ τ₁ τ₂ : v₁ :ᵥ τ₁ → v₂ :ᵥ τ₂ → ⟨ v₁, v₂ ⟩ᵥ :ᵥ (τ₁ × τ₂)
+where "v :ᵥ τ" := (type v τ).
 
 Definition with_type τ := { v | type v τ }.
 
 Notation "V⟦ τ ⟧" := (with_type τ).
+
+Theorem value_well_typed v : ∃ τ, v :ᵥ τ.
+Proof.
+   induction v.
+   - econstructor. econstructor.
+   - econstructor. econstructor.
+   - econstructor. econstructor.
+   - inversion IHv1. inversion IHv2. eexists. econstructor; eauto.
+Qed.
+
+Theorem type_deterministic v σ τ : v :ᵥ σ → v :ᵥ τ → σ = τ.
+Proof.
+   intros Hσ. generalize dependent σ. generalize dependent τ. 
+   induction v; intros; inv H; inv Hσ; try f_equal; auto.
+Qed.
