theories/Dynamics/Term.v
@@ -1,3 +1,19 @@
-From Metaconfigurations Require Import Syntax.Term Syntax.Ty Object Process.
+From Metaconfigurations Require Import Syntax.Term Syntax.Ty Syntax.Value Object Process.
+From stdpp Require Import base.
 
-Reserved Notation "⟨ e, 
+Reserved Notation "⟨ ϵ, σ, e ⟩ ⇓ v" (at level 80, no associativity).
+
+Section Eval.
+
+  Variable Π : Type.
+
+  Context `{Process Π}.
+
+  Variable Ω : Type.
+
+  Context `{Object Π Ω}.
+
+  Variable π : Π.
+
+  Inductive eval : Term.t Π Ω π → Value.t → Prop :=
+    | 
