theories/Map.v
@@ -1,0 +1,32 @@
+From stdpp Require Import base decidable.
+
+Section Map.
+
+  Variable K V : Type.
+
+  Context `{EqDecision K}.
+
+  Definition t := K → V.
+
+  Definition rebind : K → V → t → t.
+  Proof.
+    intros k v m k'. unfold EqDecision in *. destruct (decide (k = k')).
+    - exact v.
+    - exact (m k').
+  Defined.
+
+  Definition lookup (k : K) (m : t) : V := m k.
+
+  Definition with_default (d : V) : t := λ _, d.
+
+  Theorem lookup_rebind_same k v m : lookup k (rebind k v m) = v.
+  Proof.
+    unfold lookup, rebind. now destruct (decide (k = k)).
+  Qed.
+
+  Theorem lookup_rebind_diff k k' v m : k ≠ k' → lookup k' (rebind k v m) = lookup k' m.
+  Proof.
+    intros. unfold lookup, rebind. now destruct (decide (k = k')).
+  Qed.
+
+End Map.
