theories/Syntax/Term.v
@@ -1,7 +1,7 @@
 From stdpp Require Import base gmap.
 Require Import Coq.Strings.String.
 Require Import Coq.Lists.List.
-Require Import Metaconfigurations.Object.
+From Metaconfigurations Require Import Object Process.
 
 Variant bop : Set :=
   | Add
@@ -22,48 +22,19 @@ Section Term.
 
   Context `{Object Π Ω}.
 
+  Variable π : Π.
+
   Inductive t : Type :=
-    | Var (x : string)
+    | Var (x : register_names π)
     | Invoke (ω : Ω) (op : (type ω).(OP Π)) (arg : t)
     | Bop (op : bop) (e₁ : t) (e₂ : t)
     | Uop (op : uop) (e : t)
-    | Tuple (es : list t)
-    | Proj (e : t) (index : nat)
+    | Pair (e₁ : t) (e₂ : t)
+    | ProjL (e : t)
+    | ProjR (e : t)
     | Int (n : Z)
     | Bool (b : bool)
     | Unit.
-
-  Section custom_ind.
-    Variable P : t → Prop.
-    Hypothesis HVar : ∀ x, P (Var x).
-    Hypothesis HCall : ∀ ω op e, P e → P (Invoke ω op e).
-    Hypothesis HBop : ∀ op e₁ e₂, P e₁ → P e₂ → P (Bop op e₁ e₂).
-    Hypothesis HUop : ∀ op e, P e → P (Uop op e).
-    Hypothesis HTuple : ∀ es, Forall P es → P (Tuple es).
-    Hypothesis HProj : ∀ e n, P e → P (Proj e n).
-    Hypothesis HInt : ∀ n, P (Int n).
-    Hypothesis HBool : ∀ b, P (Bool b).
-    Hypothesis HUnit : P Unit.
-
-    Definition custom_ind : ∀ e, P e :=
-      fix f e : P e :=
-        let flist (es : list t) : Forall P es :=
-          list_ind
-            (Forall P) (Forall_nil P)
-            (fun e l H => Forall_cons P e l (f e) H) es
-        in      
-        match e with
-        | Var x => HVar x
-        | Invoke ω op e => HCall ω op e (f e)
-        | Bop op e₁ e₂ => HBop op e₁ e₂ (f e₁) (f e₂)
-        | Uop op e => HUop op e (f e)
-        | Tuple es => HTuple es (flist es)
-        | Proj e n => HProj e n (f e)
-        | Int n => HInt n
-        | Bool b => HBool b
-        | Unit => HUnit
-        end.
-  End custom_ind.
 
 End Term.
 
