theories/Syntax/Ty.v
@@ -5,26 +5,6 @@ Inductive t : Type :=
   | Int 
   | Bool 
   | Unit
-  | Tuple (τs : list t).
+  | Prod (σ : t) (τ : t).
 
-Section custom_ind.
-  Variable P : t → Prop.
-
-  Hypothesis HInt : P Int.
-  Hypothesis HBool : P Bool.
-  Hypothesis HUnit : P Unit.
-  Hypothesis HTuple : ∀ τs, Forall P τs → P (Tuple τs).
-
-  Definition custom_ind : ∀ τ, P τ :=
-    fix f τ : P τ :=
-      match τ with
-      | Int => HInt
-      | Bool => HBool
-      | Unit => HUnit
-      | Tuple τs =>
-        HTuple τs
-          (list_ind
-              (Forall P) (Forall_nil P)
-              (fun τ l H => Forall_cons P τ l (f τ) H) τs)
-      end.
-End custom_ind.
+Notation "τ₁ × τ₂" := (Prod τ₁ τ₂) (at level 80).
