theories/Syntax/Value.v
@@ -9,69 +9,12 @@ Inductive t :=
   | Int (n : Z)
   | Bool (b : bool)
   | Unit
-  | Tuple (vs : list t).
+  | Pair (σ : t) (τ : t).
 
-Section custom_ind.
-  Variable P : t → Set.
-  Hypothesis HInt : ∀ n, P (Int n).
-  Hypothesis HBool : ∀ b, P (Bool b).
-  Hypothesis HUnit : P Unit.
-  Hypothesis HTuple : ∀ vs, Forall P vs → P (Tuple vs).
+Coercion Int : Z >-> t.
+Coercion Bool : bool >-> t.
 
-  Definition custom_ind : ∀ v, P v :=
-    fix f v : P v :=
-      let flist (vs : list t) : Forall P vs :=
-        list_ind
-          (Forall P) (Forall_nil P)
-          (fun v l H => Forall_cons P v l (f v) H) vs
-      in      
-      match v with
-      | Int n => HInt n
-      | Bool b => HBool b
-      | Unit => HUnit
-      | Tuple vs => HTuple vs (flist vs)
-      end.
-End custom_ind.
+Notation "'⊤ᵥ'" := Unit.
 
-Lemma eq_dec (v v' : t) : decidable (v = v').
-Proof.
-  generalize dependent v'. unfold decidable. 
-  induction v using custom_ind;
-  destruct v'; auto.
-  - destruct (Z.eq_dec n n0).
-    + left. congruence.
-    + right. intuition. injection H. assumption.
-  - destruct (bool_eq_dec b b0).
-    + left. congruence.
-    + right. intuition. injection H. assumption.
-  - generalize dependent vs0. induction H.
-    + destruct vs0; auto.
-    + destruct vs0. auto. 
-      destruct (H t0), (IHForall vs0).
-      * left. congruence.
-      * right. intuition. injection H3. intros. apply H2. congruence.
-      * right. intuition. injection H3. auto.
-      * right. intuition. injection H3. auto.
-Defined.
+Notation "⟨ v₁ , v₂ ⟩ᵥ" := (Pair v₁ v₂).
 
-Check
-
-Lemma eq_dec_nst : forall n m : nat, {n = m} + {n <> m}.
-Proof.
-  intro n; induction n as [|n IHn]. intro m; destruct m as [|m].
-  - now left.
-  - now right.
-  - now right.
-  - destruct (IHn m); [left|right]; auto.
-Defined.
-
-Unset Printing Notations.
-
-Program Instance t_eqdec : EqDec (eq_setoid t) := {
-  equiv_dec :=
-    fun v v' =>
-      match eq_dec v v' with
-      | or_introl P => left P
-      | or_intror P => right P
-      end
-}.
